CoqCode/Auxiliaries.v
@@ -1,5 +1,6 @@
 Require Import Metalib.Metatheory.
 Require Import Language.
+Require Import Coq.Program.Equality.
 
 Lemma anno_equal_split :
   forall (e1 e2 : trm) (A B : typ),
@@ -8,3 +9,23 @@ Proof.
   intros.
   induction e1; inversion H; eauto.
 Qed.
+
+Lemma anno_equal_split2 :
+  forall (e1 e2 : trm) (A B : typ),
+    (e1 = e2) /\ (A = B) -> (trm_anno e1 A) = (trm_anno e2 B).
+Proof.
+  intros.
+  destruct H.
+  rewrite H0.
+  rewrite H. reflexivity.
+Qed.
+
+Lemma typing_sub_check :
+  forall (e : trm) (A B : typ),
+    typing nil nil check_mode e A ->
+    sub A B ->
+    typing nil nil check_mode e B.
+Proof.
+  intros e A B Htyp Hsub.
+  induction Htyp.
+Admitted.
