CoqCode/Deterministic.v
@@ -14,6 +14,7 @@ Proof.
   - inversion H_ord.
 Qed.
 
+
 Lemma tred_toplike :
   forall (A : typ),
     toplike A -> forall e1 e2 e1' e2' : trm, typedred e1 A e1' -> typedred e2 A e2' -> e1' = e2'.
@@ -92,16 +93,37 @@ Proof.
     apply sub_and_l.
     eapply IHHred. constructor. assumption.
     inversion H8; subst.
-    Focus 2.
+    + inversion H3.
     + apply typing_anno. constructor. assumption.
-Admitted.
-  (* pose proof (tred_to_sub e1 e1' A0 A) as Hsub1. *)
-  (* apply Hsub1. assumption. assumption. assumption. *)
-  (* pose proof (tred_to_sub e2 e2' A0 B) as Hsub2. *)
-  (* apply Hsub2. assumption. assumption. assumption. *)
-  (* apply tred_toplike with (A:=A0) (e1:=e1) (e2:=e2). *)
-(*   (* assumption. assumption. assumption. *) *)
-(* Qed. *)
+  - intros B0 Htyp.
+    inversion Htyp; subst; clear Htyp.
+    inversion H7; subst; clear H7.
+    apply sub_and_r.
+    eapply IHHred. constructor. assumption.
+    inversion H8; subst.
+    + inversion H3.
+    + apply typing_anno. constructor. assumption.
+Qed.
+
+Lemma disjoint_value_consistent :
+  forall (A B : typ) (v1 v2 : trm),
+    disjoint_spec A B -> value v1 -> value v2 ->
+    typing nil nil infer_mode v1 A ->
+    typing nil nil infer_mode v2 B ->
+    consistency_spec v1 v2.
+Proof.
+  intros A B v1 v2 Hdis Hv1 Hv2 Htyp1 Htyp2.
+  unfold consistency_spec.
+  intros A0 e1' e2'. intros Hred1 Hred2.
+  assert (Hsub1: sub A A0).
+  eapply tred_sub. apply Hv1. apply Hred1. apply Htyp1.
+  assert (Hsub2: sub B A0).
+  eapply tred_sub. apply Hv2. apply Hred2. apply Htyp2.
+  assert (Htop : toplike A0).
+  unfold disjoint_spec in Hdis.
+  apply Hdis. assumption. assumption.
+  eapply tred_toplike. apply Htop. apply Hred1. apply Hred2.
+Qed.
 
 Lemma tred_determinism :
   forall (v v1 v2 : trm) (A : typ),
@@ -132,25 +154,89 @@ Proof.
     + eapply IHHred1.
       * constructor. assumption.
       * destruct Htyp. inversion H3; subst.
-        inversion H14; subst.
-        inversion H4; subst.
-        inversion H5; subst.
-        unfold disjoint_spec in H15.
-    (* + assert (Hval1 : value (trm_anno p1 A)). constructor. assumption. *)
-    (*   eapply IHHred1 in Hval1. apply Hval1. *)
-Admitted.
+        inversion H14; subst. inversion H4.
+        exists A. eapply typing_anno. constructor. assumption.
+      * assumption.
+    + destruct Htyp. inversion H3; subst. inversion H14; subst; clear H14. inversion H4.
+      assert(Hcons: consistency_spec (trm_anno p1 A) (trm_anno p2 B)).
+      eapply disjoint_value_consistent; eauto 3.
+      unfold consistency_spec in Hcons.
+      eapply Hcons. apply Hred1. apply H12.
+    + inversion H2.
+  - intros v2 Hred2.
+    inversion Hred2; subst; eauto.
+    + eapply tred_ord_toplike; eauto 3.
+    + destruct Htyp. inversion H3; subst. inversion H14; subst; clear H14. inversion H4.
+      assert(Hcons: consistency_spec (trm_anno p1 A) (trm_anno p2 B)).
+      eapply disjoint_value_consistent; eauto 3.
+      unfold consistency_spec in Hcons.
+      symmetry.
+      eapply Hcons. apply H12. apply Hred1.
+    + eapply IHHred1.
+      * constructor. assumption.
+      * destruct Htyp. inversion H3; subst.
+        inversion H14; subst. inversion H4.
+        exists B. eapply typing_anno. constructor. assumption.
+      * assumption.
+    + inversion H2.
+  - intros v2 Hred2.
+    inversion Hred2; subst; clear Hred2.
+    + inversion H4.
+    + inversion H10.
+    + inversion H10.
+    + assert (Heq1: (trm_anno p1 D) = (trm_anno p0 D0)).
+      eapply IHHred1_1; eauto 3.
+      assert (Heq2: (trm_anno p2 E) = (trm_anno p3 E0)).
+      eapply IHHred1_2; eauto 3.
+      eapply anno_equal_split in Heq1. destruct Heq1 as [Heq11 Heq12].
+      eapply anno_equal_split in Heq2. destruct Heq2 as [Heq21 Heq22].
+      rewrite Heq11. rewrite Heq12. rewrite Heq21. rewrite Heq22.
+      reflexivity.
+Qed.
+
+Lemma tred_value :
+  forall (v v' : trm) (A : typ),
+    value v -> typedred v A v' -> value v'.
+Proof.
+  intros v v' A Hval Hred.
+  induction Hred; eauto.
+Qed.
+
+Lemma tred_typing :
+  forall (v v' : trm) (A : typ),
+    value v ->
+    (exists (B : typ), typing nil nil infer_mode v B) ->
+    typedred v A v' ->
+    (exists (C : typ), typing nil nil infer_mode v' C).
+Proof.
+  intros v v' A Hval Htyp Hred.
+  induction Hred; eauto.
+  - destruct Htyp.
+    inversion H2; subst. inversion H7; subst.
+    exists (typ_arrow A D). apply typing_anno; eauto 3.
 
 Lemma papp_determinism :
   forall (v1 v2 e1 e2 : trm),
+    value v1 -> value v2 ->
+    (exists (A : typ), typing nil nil infer_mode v1 A) ->
+    (exists (B : typ), typing nil nil infer_mode v2 B) ->
     papp v1 v2 e1 -> papp v1 v2 e2 -> e1 = e2.
 Proof.
-  intros v1 v2 e1 e2 Hp1.
+  intros v1 v2 e1 e2 Hval1 Hval2 Htyp1 Htyp2 Hp1.
   generalize dependent e2.
   induction Hp1.
   - intros e2 Hp2. inversion Hp2. reflexivity.
   - intros e2 Hp2. inversion Hp2. reflexivity.
   - intros e2 Hp2. inversion Hp2; subst.
-    Admitted.
+    assert (Hequal: v' = v'0).
+    eapply tred_determinism; eauto 3.
+    rewrite Hequal. reflexivity.
+  - intros e2 Hp2. inversion Hp2; subst; clear Hp2.
+    apply IHHp1.
+    + eapply tred_value. apply Hval1. apply H0.
+    + apply Hval2.
+    +
+
 
 Lemma step_determinism :
   forall (e e1 e2 : trm) (A : typ),
