CoqCode/Notations.v
@@ -18,3 +18,4 @@ Notation "T S ⊢ e ⇒ A" := (typing T S infer_mode e A) (at level 50).
 Notation "T S ⊢ e ⇐ A" := (typing T S check_mode e A) (at level 50).
 
 Notation "e ~-> e'" := (step e e') (at level 68).
+Notation "v ◐ vl ~-> e" := (papp v vl e) (at level 69).
